\documentclass[11pt,a4paper]{jsarticle}
\usepackage[dvips]{graphicx}
\usepackage{fancyhdr}
\usepackage{here}
\setcounter{page}{0}
%
\begin{document}

\pagestyle{empty}
\thispagestyle{empty}
\frac{s + 2\xi\omega_n^2}{s^2+2\xi \omega_n s +\omega_n^2} \right)
  \end{equation}
  となる．これを逆ラプラス変換して以下の式を求める．
  \begin{equation}
   y(t) = y_0 \left( 1-\frac{1}{\sqrt{1-\xi^2}}e^{-\beta t} \cos{(\gamma t-\delta)} \right)
  \end{equation}
  また，$\omega_n = \sqrt{a_0},\ \xi = \frac{a_1}{2\sqrt{a_0}},\ \beta = \xi \omega_n,\ \gamma = \omega_n \sqrt{1-\xi^2},\ \delta = \tan^{-1} \left(\frac{\xi}{\sqrt{1-\xi^2}} \typeout{=== Region from (point) to (mark) ===}

\end{document}
